theories/Invariant.v
@@ -1,0 +1,184 @@
+Require Import Coqlib.
+Require Import Universe.
+Require Import STS.
+Require Import Behavior.
+Require Import ModSem.
+Require Import Skeleton.
+Require Import PCM.
+Require Import HoareDef.
+Require Import TODOYJ.
+Require Import ProofMode.
+Require Import HTactics.
+Require Import STB.
+
+Set Implicit Arguments.
+
+
+
+
+
+
+
+Section AUX.
+  Definition invRA: URA.t := Excl.t unit.
+
+  Definition inv_token: (@URA.car invRA) := Some tt.
+
+  Context `{Σ: GRA.t}.
+  Context `{@GRA.inG invRA Σ}.
+
+  Definition inv_closed: iProp := OwnM inv_token%I.
+
+  Lemma inv_closed_unique
+    :
+      inv_closed -∗ inv_closed -∗ False
+  .
+  Proof.
+    unfold inv_closed, inv_token.
+    iIntros "H0 H1".
+    iCombine "H0 H1" as "H". iOwnWf "H" as WF. exfalso.
+    repeat ur in WF. ss.
+  Qed.
+
+  Definition inv_le
+             A (le: A -> A -> Prop)
+    :
+      (A + Any.t * Any.t) -> (A + Any.t * Any.t) -> Prop :=
+    fun x0 x1 =>
+      match x0, x1 with
+      | inl a0, inl a1 => le a0 a1
+      | inr st0, inr st1 => st0 = st1
+      | _, _ => False
+      end.
+
+  Lemma inv_le_PreOrder A (le: A -> A -> Prop)
+        (PREORDER: PreOrder le)
+    :
+      PreOrder (inv_le le).
+  Proof.
+    econs.
+    { ii. destruct x; ss. refl. }
+    { ii. destruct x, y, z; ss.
+      { etrans; et. }
+      { subst. auto. }
+    }
+  Qed.
+
+  Definition inv_wf
+             A
+             (R_src: A -> Any.t -> Any.t -> iProp)
+             (R_tgt: A -> Any.t -> Any.t -> iProp)
+    : _ -> (((Σ * Any.t)) * ((Σ * Any.t)) -> Prop) :=
+    @mk_wf
+      _
+      (A + Any.t * Any.t)
+      (fun a' mp_src mp_tgt =>
+         match a' with
+         | inl a => R_src a mp_src mp_tgt
+         | inr (mp_src1, mp_tgt1) => inv_closed ** ⌜mp_src1 = mp_src /\ mp_tgt1 = mp_tgt⌝
+         end)%I
+      (fun a' mp_src mp_tgt =>
+         match a' with
+         | inl a => R_tgt a mp_src mp_tgt
+         | inr (mp_src, mp_tgt) => top1
+         end)
+  .
+
+  Definition mk_fspec_inv (fsp: fspec): fspec :=
+    @mk_fspec
+      _
+      (meta fsp)
+      (fun mn x varg_src varg_tgt o =>
+         inv_closed ** (precond fsp) mn x varg_src varg_tgt o)
+      (fun mn x vret_src vret_tgt =>
+         inv_closed ** (postcond fsp) mn x vret_src vret_tgt).
+
+  Lemma fspec_weaker_fspec_inv_weakker (fsp0 fsp1: fspec)
+        (WEAKER: fspec_weaker fsp0 fsp1)
+    :
+      fspec_weaker (mk_fspec_inv fsp0) (mk_fspec_inv fsp1).
+  Proof.
+    ii. exploit WEAKER. i. des. exists x_tgt. split; ss.
+    { ii. iIntros "[INV H]". iSplitL "INV"; ss.
+      iApply PRE. iExact "H". }
+    { ii. iIntros "[INV H]". iSplitL "INV"; ss.
+      iApply POST. iExact "H". }
+  Qed.
+
+End AUX.
+
+Ltac iarg :=
+  let PRE := constr:("PRE") in
+  let INV := constr:("INV") in
+  let CLOSED := constr:("☃CLOSED") in
+  eapply (@harg_clo _ _ _ PRE INV);
+  [eassumption
+  |
+  ];
+  i;
+  mDesSep PRE as CLOSED PRE;
+  match goal with
+  | [ |- (gpaco7 _ _ _ _ _ _ _ _ ?w _ _)] =>
+    destruct w as [?|[?mp_src ?mp_tgt]]; simpl;
+    [
+        |mAssertPure False; ss; iDestruct "INV" as "[INV _]"; iApply (inv_closed_unique with "☃CLOSED INV")
+    ]
+  end.
+
+Tactic Notation "icall_open" uconstr(o) uconstr(x) "with" constr(Hns) :=
+  let POST := get_fresh_name_tac "POST" in
+  let INV := constr:("☃CLOSED") in
+  let Hns := select_ihyps Hns in
+  let Hns := constr:("☃CLOSED"::Hns) in
+  eapply (@hcall_clo _ _ Hns POST INV o _ x _ (inr (_, _)));
+  unshelve_goal;
+  [eassumption
+  |
+  |start_ipm_proof; iSplitL "☃CLOSED"; [iModIntro; iSplitL "☃CLOSED"; [iExact "☃CLOSED"|ss]|]
+  |eauto with ord_step
+  |
+  |
+  on_current ltac:(fun H => try clear H);
+  intros ? ? ? ? ? ? [|[?mp_src ?mp_tgt]]; i; simpl;
+  on_current ltac:(fun H => simpl in H);
+  [exfalso; match goal with | H: inv_le _ _ _ |- _ => cbn in H; inv H end
+  |mDesSep "☃CLOSED" as "☃CLOSED" "☃TMP"; mPure "☃TMP" as [[] []]
+  ]
+  ].
+
+Tactic Notation "icall_weaken" uconstr(ftsp) uconstr(o) uconstr(x) uconstr(a) "with" constr(Hns) :=
+  let POST := get_fresh_name_tac "POST" in
+  let INV := get_fresh_name_tac "INV" in
+  let CLOSED := constr:("☃CLOSED") in
+  let TMP := constr:("☃TMP") in
+  let Hns := select_ihyps Hns in
+  let Hns := constr:("☃CLOSED"::Hns) in
+  eapply (@hcall_clo_weaken _ _ Hns POST INV ftsp o x _ (inl a));
+  unshelve_goal;
+  [|
+   eassumption
+   |
+   |start_ipm_proof; iFrame "☃CLOSED"
+   |eauto with ord_step
+   |
+   |on_current ltac:(fun H => try clear H);
+    intros ? ? ? ? ? ? [|[?mp_src ?mp_tgt]]; i; simpl;
+    on_current ltac:(fun H => simpl in H);
+    [
+      mDesSep POST as "☃CLOSED" POST
+    |
+    mDesSep INV as "☃CLOSED" INV;
+    mDesSep POST as "☃TMP" POST;
+    mAssertPure False; [iApply (inv_closed_unique with "☃TMP ☃CLOSED")|ss]
+    ]
+  ].
+
+Tactic Notation "iret" uconstr(a) :=
+  eapply (@hret_clo _ _ _ (inl a)); unshelve_goal;
+  [eauto with ord_step
+  |eassumption
+  |
+  |
+  |start_ipm_proof; iFrame "☃CLOSED"
+  |
+  ].
